src/tls/test/TestDH.fst
@@ -8,7 +8,7 @@ open TLSConstants
 let main () : ML unit =
   let g = default_group in
   let gx = keygen g in
-  let gy, gxy = dh_responder #g gx in
+  let gy, gxy = dh_responder #g (pubshare gx) in
   let gxy' = dh_initiator #g gx gy in
   let gxy  = hex_of_bytes gxy in
   let gxy' = hex_of_bytes gxy' in
